% !TeX encoding = UTF-8
% !TeX root = main.tex

Try to get saPAKE \cite{EC:JarKraXu18}.
Hash function $H:\bits^* \to \Zq^m$.
\begin{figure}
    \centering
    \fbox{
        \begin{tabular}{lcl}
        \textbf{Client} $\Client(\pw)$ & & \textbf{Server} $\Server()$\\ \hdashline
         & Public Setup & \\ 
         & $\matA\gets\Zq^{n \times m}$ & \\ \hdashline
         & Store Password File&   \\ 
         & & $(\matC,\matT)\gets\TrapGen(n,m)$  \\ 
        & \LLarrow[16]{$\matC$}&\\
        $\vecs\gets\Zq^m$ & &\\
        $\vece\gets \errorDist^n, e'\gets\errorDist$ & &\\
        $\ct_1 = \colCA\vecs+\vece$ & &\\
        $\ct_2 = H(\pw)^\top\vecs+e'+\mu\cdot\qhalf$ & &\\
        $\ct_3 = H'(\pw,\mu)\oplus \akekey$ \codecomment{$\akekey$ will be the AKE keys}& &\\
         & \LRarrow[16]{$\ct=(\ct_1,\ct_2,\ct_3)$} & store $\ct$\\ \hdashline
          & Password Authentication & \\
        $\vecx\gets\errorDist^n$& &\\
        $\vect=H(\pw)^\top + \vecx^\top\matA$ & & \\
         & \LRarrow[16]{$\vect$} & \\ 
         & & $\vecy\gets\SamplePre(\matC,\matT,\vect)$\\
         &\LLarrow[16]{$(\vecy,\ct)$} & \\
        parse $(\ct_1,\ct_2,\ct_3)=\ct$ & & \\
        Round $\ct_2-(\vecy^\top,\vecx^\top)\ct_1$ to get $\mu$& & \\
        $\akekey\gets H(\pw,\mu) \oplus \ct_3$ & & \\
        Derive AKE keys from $\akekey$ & \fbox{AKE} & 
        \end{tabular}
    }
    
    \caption{Lattice OPAQUE.}
    \label{fig:protocol}
\end{figure}

\paragraph{Correctness}
\begin{align*}
    \ct_2-(\vecy^\top,\vecx^\top)\ct_1 &=\ct_2 - (\vecy^\top,\vecx^\top)(\colCA\vecs+\vece)\\
    &=\ct_2 - ((\vecy^\top,\vecx^\top)\colCA\vecs+(\vecy^\top,\vecx^\top)\vece)\\
    &= \ct_2- ((\vecy^\top\matC-\vecx^\top\matA)\vecs + (\vecy^\top,\vecx^\top)\vece)\\
    &= \ct_2 - ((\vect-\vecx^\top\matA)\vecs + (\vecy^\top,\vecx^\top)\vece)\\
    &=\ct_2 - (\vect\vecs-\vecx^\top\matA\vecs + (\vecy^\top,\vecx^\top)\vece)\\
    &=\ct_2 - (H(\pw)^\top\vecs + \vecx^\top\matA\vecs-\vecx^\top\matA\vecs + (\vecy^\top,\vecx^\top)\vece)\\
    &=\ct_2 - (H(\pw)^\top\vecs + (\vecy^\top,\vecx^\top)\vece)\\
    &=H(\pw)^\top\vecs+e'+\mu\cdot\qhalf -(H(\pw)^\top\vecs + (\vecy^\top,\vecx^\top)\vece) \\
    &=\underbrace{e'}_{\text{short}}+\mu\cdot\qhalf \underbrace{-  (\vecy^\top,\vecx^\top)\vece}_{\text{short}} \\
\end{align*}